\newpage
\hypertarget{nfsft}{}
{\color{blue} NFSFT}
\vfill
nonuniform fast Fourier transform on the sphere
\begin{equation*}
  f\left(\zb {\xi}_d\right)=\sum\limits_{k=0}^{M} \sum\limits_{n=-k}^{k} {\hat
  f}_k^n \; Y_k^n\left(\zb {\xi}_d\right)\,, \qquad d =0,\ldots,D-1
\end{equation*}
in ${\cal O}(M^2 \log^2 M + |\log\varepsilon|^2D)$
\vfill
matrix-vector notation: $\zb f=\zb A \zb {\hat f}$ where
\begin{equation*}
\zb A=\left(Y_k^n\left(\theta_d,\phi_d\right)\right)_
{d=0,\hdots,D-1;\,k=0,\hdots,M; |n| \le k} \in \mathbb{C}^{D \times \left(M+1\right)^2}
\end{equation*}
and $Y_k^n(\theta,\phi)=P_k^{|n|}(\cos\theta) \e^{\ti n\phi}$
\vfill
applications: geophysics, tomography, crystallography
\vfill

\newpage
{\color{blue} NFSFT}
\vfill
torus $\mathbb{T}^2$ vs. sphere $\mathbb{S}^2$, square matrix $\zb A$,
\begin{center}
 \begin{tabular}{c c}
  FFT                      & FSFT\\
  {\tiny (Cooley, Tukey 1965; Frigo, Johnson 1997-)}         &
  {\tiny(Driscoll, Healy, Rockmore 1994-; Potts, Steidl, Tasche 1998;}\\ &
  {\tiny Mohlenkamp 1999; Suda, Takami 2001}\\[1.5ex]
  NFFT                   & NFSFT\\
  %${\cal{O}}\left(M^2\log M + \log^2\left(1/\varepsilon\right)M^2\right)$ &
  %${\cal{O}}\left(M^2\log^2 M + \log^2\left(1/\varepsilon\right)M^2\right)$\\
  {\tiny(Dutt, Rokhlin 1993; Beylkin 1995-; Steidl 1997-;} &
  {\tiny (Keiner, K., Potts 2002-)}\\ 
  {\tiny Greengard, Lee 2004; K., Potts 2002-)} & \\[1.5ex]
  ${\cal{O}}\left(M^2 \log M\right)$ & ${\cal{O}}\left(M^2 \log^2 M\right)$\\
 \end{tabular}
\end{center}
\vfill
knots on $\mathbb{S}^2$
\begin{center}
 \begin{tabular}{c c c}
   \includegraphics[width=5cm,height=5cm,keepaspectratio]{pics/scattered.jpg}
   &
   \includegraphics[width=5cm,height=5cm,keepaspectratio]{pics/grid.jpg}
   &
   \includegraphics[width=5cm,height=5cm,keepaspectratio]{pics/equi_grid.jpg}\\
   ${\cal{O}}\left(M^4\right)$ & ${\cal{O}}\left(M^3\right)$ &
   ${\cal{O}}\left(M^2 \log^2 M\right)$
 \end{tabular}
\end{center}
\vfill

\newpage
{\color{blue} NFSFT}
\vfill
\begin{enumerate}
\item given $\zb {\hat f} \in \mathbb{C}^{(M+1)^2}$ in
  \begin{equation*}
    f\left(\theta,\phi\right)=
    \sum_{k=0}^M \sum_{n=-k}^k {\hat f}_k^n Y_k^n\left(\theta,
        \phi\right),
  \end{equation*}
  %where $Y_k^n\left(\theta,
  %\phi\right)=P_k^{|n|}\left(\cos\left(\theta\right)\right)\e^{\ti n\phi}$,
\item compute $\zb a \in \mathbb{C}^{(2M+1)(M+1)}$ in
  \begin{equation*}   
    f\left(\theta,\phi\right)=
    \sum_{n=-M}^M \sum_{k=0}^M a_{k}^n \, t_k^n\left(\theta\right)
    \e^{\ti n\phi}
  \end{equation*}
  where $t_k^n\left(\theta\right)= (\sin\theta)^{\delta_{n\%2}} \, T_k\left(\cos\theta\right)$,
\item compute $\zb c \in \mathbb{C}^{(2M+1)^2}$ in
  \begin{equation*}
    f \left( \theta , \phi\right)=
    \sum_{n=-M}^{M} \sum_{k=-M}^{M} c_k^n \e^{\ti k\theta} \e^{\ti n\phi}
  \end{equation*}
\item compute $\zb f\in \mathbb{C}^D, \;f_d =f ( \theta_d , \phi_d)$ by $2d$-NFFT
\end{enumerate}
\vfill

\newpage
{\color{blue} NFSFT}
\vfill
remaining task
\begin{equation*}
 h_n\left(\cos\theta_s\right)=
 \sum_{k=|n|}^M {\hat f}_k^n P_k^{|n|}\left(\cos\theta_s\right),
\end{equation*}
using the three-term recurrence relation, Clenshaw algorithm, ${\cal{O}}\left(M^2\right)$
  \begin{eqnarray*}
   {\color{Green}a_{k+1}^n} P_{{\color{Red}k+1}}^n\left(x\right) & \mapsto &
   {\color{Green}\left(a_{k+1}^n\left(\alpha_k^nx+\beta_k^n\right)+a_{k}^n\right)}P_{{\color{Red}k}}^n\left(x\right),\\
   & & {\color{Green}\left(a_{k+1}^n\gamma_k^n+a_{k-1}^n\right)}P_{{\color{Red}k-1}}^n\left(x\right)
  \end{eqnarray*}
using a generalised three-term recurrence relation and a tree-like organisation, fast polynom transform, ${\cal{O}}\left(M \log^2 M\right)$
  \begin{eqnarray*}
  {\color{Green}a_{k+c}^{\left(\tau\right)}\left(x\right)} P_{{\color{Red}k+c}}^n \left(x\right) & \mapsto &
  \overbrace{\left(a_{k+c}^{\left(\tau\right)}\left(x\right)P_{c}^n \left(x,k\right)+a_{k}^{\left(\tau\right)}\left(x\right)\right)}^{{\color{Green}a_{k}^{\left(\tau+1\right)}\left(x\right)}} P_{{\color{Red}k}}^n \left(x\right),\\
  & &\underbrace{\left(a_{k+c}^{\left(\tau\right)}\left(x\right)\gamma_{k}^n P_{c-1}^n \left(x,k+1\right) +
    a_{k-1}^{\left(\tau\right)}\left(x\right)\right)}_{{\color{Green}a_{k-1}^{\left(\tau+1\right)}\left(x\right)}} P_{{\color{Red}k-1}}^n \left(x\right)
  \end{eqnarray*}
\vfill

%%% Local Variables: 
%%% mode: latex
%%% TeX-master: "vortrag"
%%% End: 
